src/Narcissus/Examples/NetworkStack/bench.sh
@@ -1,7 +1,7 @@
 #!/usr/bin/env sh
 ocamlopt -config
-# cp ../../../../Fiat4Mirage.ml ./
+cp ../../../../Fiat4Mirage.ml ./
 rm -f Fiat4Mirage.mli
-ocamlfind ocamlopt -p -g -linkpkg -thread -package core -package core_bench Int64Word.ml ArrayVector.ml OCamlNativeInt.ml Fiat4Mirage.ml bench.ml -o fiat4mirage-bench || exit 1
+ocamlfind ocamlopt -p -g -linkpkg -thread -package cstruct -package core -package core_bench Int64Word.ml ArrayVector.ml CstructBytestring.ml OCamlNativeInt.ml Fiat4Mirage.ml bench.ml -o fiat4mirage-bench || exit 1
 ./fiat4mirage-bench -width 2000 -quota 5 -ci-absolute +time
 #short, tall, line, blank or column
